lib/coq/Sail2_state_lemmas.v
@@ -1,0 +1,722 @@
+Require Import Sail2_values Sail2_prompt_monad Sail2_prompt Sail2_state_monad Sail2_state Sail2_state Sail2_state_lifting.
+Require Import Sail2_state_monad_lemmas.
+
+(* Monad lifting *)
+
+Lemma liftState_bind Regval Regs A B E {r : Sail2_values.register_accessors Regs Regval} {m : monad Regval A E} {f : A -> monad Regval B E} {s} :
+  liftState r (bind m f) s = bindS (liftState r m) (fun x => liftState r (f x)) s.
+revert s. induction m; simpl.
+all: try (intros; unfold seqS; rewrite bindS_assoc; auto using bindS_ext_cong).
+all: try auto.
+* intro s.
+  rewrite bindS_returnS_left.
+  reflexivity.
+Qed.
+Hint Rewrite liftState_bind : liftState.
+
+Lemma liftState_return Regval Regs A E {r : Sail2_values.register_accessors Regs Regval} {a :A} :
+  liftState (E:=E) r (returnm a) = returnS a.
+reflexivity.
+Qed.
+Hint Rewrite liftState_return : liftState.
+
+(*
+Lemma Value_liftState_Run:
+  List.In (Value a, s') (liftState r m s)
+  exists t, Run m t a.
+  by (use assms in \<open>induction r m arbitrary: s s' rule: liftState.induct\<close>;
+      simp add: failS_def throwS_def returnS_def del: read_regvalS.simps;
+      blast elim: Value_bindS_elim)
+
+lemmas liftState_if_distrib[liftState_simp] = if_distrib[where f = "liftState ra" for ra]
+*)
+Lemma liftState_if_distrib {Regs Regval A E r x y} {c : bool} :
+  @liftState Regs Regval A E r (if c then x else y) = if c then liftState r x else liftState r y.
+destruct c; reflexivity.
+Qed.
+Lemma liftState_if_distrib_sumbool {Regs Regval A E P Q r x y} {c : sumbool P Q} :
+  @liftState Regs Regval A E r (if c then x else y) = if c then liftState r x else liftState r y.
+destruct c; reflexivity.
+Qed.
+
+Lemma Value_bindS_iff {Regs A B E} {f : A -> monadS Regs B E} {b m s s''} :
+  List.In (Value b, s'') (bindS m f s) <-> (exists a s', List.In (Value a, s') (m s) /\ List.In (Value b, s'') (f a s')).
+split.
+* intro H.
+  apply bindS_cases in H.
+  destruct H as [(? & ? & ? & [= <-] & ? & ?) | [(? & [= <-] & ?) | (? & ? & ? & [= <-] & ? & ?)]];
+  eauto.
+* intros (? & ? & ? & ?).
+  eauto with bindS_intros.
+Qed.
+
+Lemma Ex_bindS_iff {Regs A B E} {f : A -> monadS Regs B E} {m e s s''} :
+  List.In (Ex e, s'') (bindS m f s) <-> List.In (Ex e, s'') (m s) \/ (exists a s', List.In (Value a, s') (m s) /\ List.In (Ex e, s'') (f a s')).
+split.
+* intro H.
+  apply bindS_cases in H.
+  destruct H as [(? & ? & ? & [= <-] & ? & ?) | [(? & [= <-] & ?) | (? & ? & ? & [= <-] & ? & ?)]];
+  eauto.
+* intros [H | (? & ? & H1 & H2)];
+  eauto with bindS_intros.
+Qed.
+
+Lemma liftState_throw Regs Regval A E {r} {e : E} :
+  @liftState Regval Regs A E r (throw e) = throwS e.
+reflexivity.
+Qed.
+Lemma liftState_assert Regs Regval E {r c msg} :
+  @liftState Regval Regs _ E r (assert_exp c msg) = assert_expS c msg.
+destruct c; reflexivity.
+Qed.
+Lemma liftState_exit Regs Regval A E r :
+  @liftState Regval Regs A E r (exit tt) = exitS tt.
+reflexivity.
+Qed.
+Lemma liftState_exclResult Regs Regval E r :
+  @liftState Regs Regval _ E r (excl_result tt) = excl_resultS tt.
+reflexivity.
+Qed.
+Lemma liftState_barrier Regs Regval E r bk :
+  @liftState Regs Regval _ E r (barrier bk) = returnS tt.
+reflexivity.
+Qed.
+Lemma liftState_footprint Regs Regval E r :
+  @liftState Regs Regval _ E r (footprint tt) = returnS tt.
+reflexivity.
+Qed.
+Lemma liftState_choose_bool Regs Regval E r descr :
+  @liftState Regs Regval _ E r (choose_bool descr) = choose_boolS tt.
+reflexivity.
+Qed.
+(*declare undefined_boolS_def[simp]*)
+Lemma liftState_undefined Regs Regval E r :
+  @liftState Regs Regval _ E r (undefined_bool tt) = undefined_boolS tt.
+reflexivity.
+Qed.
+Lemma liftState_maybe_fail Regs Regval A E r msg x :
+  @liftState Regs Regval A E r (maybe_fail msg x) = maybe_failS msg x.
+destruct x; reflexivity.
+Qed.
+Lemma liftState_and_boolM Regs Regval E r x y s :
+  @liftState Regs Regval _ E r (and_boolM x y) s = and_boolS (liftState r x) (liftState r y) s.
+unfold and_boolM, and_boolS.
+rewrite liftState_bind.
+apply bindS_ext_cong; auto.
+intros. rewrite liftState_if_distrib.
+reflexivity.
+Qed.
+Lemma liftState_and_boolMP Regs Regval E P Q R r x y s H :
+  @liftState Regs Regval _ E r (@and_boolMP _ _ P Q R x y H) s = and_boolSP (liftState r x) (liftState r y) s.
+unfold and_boolMP, and_boolSP.
+rewrite liftState_bind.
+simpl.
+apply bindS_ext_cong; auto.
+intros [[|] [A]] s' ?.
+* rewrite liftState_bind;
+  simpl;
+  apply bindS_ext_cong; auto;
+  intros [a' A'] s'' ?;
+  rewrite liftState_return;
+  reflexivity.
+* rewrite liftState_return.
+  reflexivity.
+Qed.
+
+Lemma liftState_or_boolM Regs Regval E r x y s :
+  @liftState Regs Regval _ E r (or_boolM x y) s = or_boolS (liftState r x) (liftState r y) s.
+unfold or_boolM, or_boolS.
+rewrite liftState_bind.
+apply bindS_ext_cong; auto.
+intros. rewrite liftState_if_distrib.
+reflexivity.
+Qed.
+Lemma liftState_or_boolMP Regs Regval E P Q R r x y s H :
+  @liftState Regs Regval _ E r (@or_boolMP _ _ P Q R x y H) s = or_boolSP (liftState r x) (liftState r y) s.
+unfold or_boolMP, or_boolSP.
+rewrite liftState_bind.
+simpl.
+apply bindS_ext_cong; auto.
+intros [[|] [A]] s' ?.
+* rewrite liftState_return.
+  reflexivity.
+* rewrite liftState_bind;
+  simpl;
+  apply bindS_ext_cong; auto;
+  intros [a' A'] s'' ?;
+  rewrite liftState_return;
+  reflexivity.
+Qed.
+Hint Rewrite liftState_throw liftState_assert liftState_exit liftState_exclResult
+             liftState_barrier liftState_footprint liftState_choose_bool
+             liftState_undefined liftState_maybe_fail
+             liftState_and_boolM liftState_and_boolMP
+             liftState_or_boolM liftState_or_boolMP
+           : liftState.
+
+Lemma liftState_try_catch Regs Regval A E1 E2 r m h s :
+  @liftState Regs Regval A E2 r (try_catch (E1 := E1) m h) s = try_catchS (liftState r m) (fun e => liftState r (h e)) s.
+revert s.
+induction m; intros; simpl;
+try solve
+[ auto
+| unfold seqS;
+  erewrite try_catchS_bindS_no_throw; intros;
+  only 2,3: (autorewrite with ignore_throw; reflexivity);
+  apply bindS_ext_cong; auto
+].
+rewrite try_catchS_throwS. reflexivity.
+Qed.
+Hint Rewrite liftState_try_catch : liftState.
+
+Lemma liftState_early_return Regs Regval A R E r x :
+  liftState (Regs := Regs) r (@early_return Regval A R E x) = early_returnS x.
+reflexivity.
+Qed.
+Hint Rewrite liftState_early_return : liftState.
+
+Lemma liftState_catch_early_return (*[liftState_simp]:*) Regs Regval A E r m s :
+  liftState (Regs := Regs) r (@catch_early_return Regval A E m) s = catch_early_returnS (liftState r m) s.
+unfold catch_early_return, catch_early_returnS.
+autorewrite with liftState.
+apply try_catchS_cong; auto.
+intros [a | e] s'; auto.
+Qed.
+Hint Rewrite liftState_catch_early_return : liftState.
+
+Lemma liftState_liftR Regs Regval A R E r m s :
+  liftState (Regs := Regs) r (@liftR Regval A R E m) s = liftRS (liftState r m) s.
+unfold liftR, liftRS. autorewrite with liftState.
+apply try_catchS_cong; auto.
+Qed.
+Hint Rewrite liftState_liftR : liftState.
+
+Lemma liftState_try_catchR Regs Regval A R E1 E2 r m h s :
+  liftState (Regs := Regs) r (@try_catchR Regval A R E1 E2 m h) s = try_catchRS (liftState r m) (fun x => liftState r (h x)) s.
+unfold try_catchR, try_catchRS. autorewrite with liftState.
+apply try_catchS_cong; auto.
+intros [r' | e] s'; auto.
+Qed.
+Hint Rewrite liftState_try_catchR : liftState.
+(*
+Lemma liftState_bool_of_bitU_nondet Regs Regval :
+  "liftState r (bool_of_bitU_nondet b) = bool_of_bitU_nondetS b"
+  by (cases b; auto simp: bool_of_bitU_nondet_def bool_of_bitU_nondetS_def liftState_simp)
+Hint Rewrite liftState_bool_of_bitU_nondet : liftState.
+*)
+Lemma liftState_read_memt Regs Regval A B E H rk a sz r s :
+  liftState (Regs := Regs) r (@read_memt Regval A B E H rk a sz) s = read_memtS rk a sz s.
+unfold read_memt, read_memt_bytes, read_memtS, maybe_failS. simpl.
+apply bindS_ext_cong; auto.
+intros [byte bit] s' valIn.
+destruct (option_map _); auto.
+Qed.
+Hint Rewrite liftState_read_memt : liftState.
+
+Lemma liftState_read_mem Regs Regval A B E H rk asz a sz r s :
+  liftState (Regs := Regs) r (@read_mem Regval A B E H rk asz a sz) s = read_memS rk a sz s.
+unfold read_mem, read_memS, read_memtS. simpl.
+unfold read_mem_bytesS, read_memt_bytesS.
+repeat rewrite bindS_assoc.
+apply bindS_ext_cong; auto.
+intros [ bytes | ] s' valIn; auto. simpl.
+apply bindS_ext_cong; auto.
+intros [byte bit] s'' valIn'.
+rewrite bindS_returnS_left. autorewrite with liftState.
+destruct (option_map _); auto.
+Qed.
+Hint Rewrite liftState_read_mem : liftState.
+
+Lemma liftState_write_mem_ea Regs Regval A E rk asz a sz r :
+  liftState (Regs := Regs) r (@write_mem_ea Regval A E rk asz a sz) = returnS tt.
+reflexivity.
+Qed.
+Hint Rewrite liftState_write_mem_ea : liftState.
+
+Lemma liftState_write_memt Regs Regval A B E wk addr sz v t r :
+  liftState (Regs := Regs) r (@write_memt Regval A B E wk addr sz v t) = write_memtS wk addr sz v t.
+unfold write_memt, write_memtS.
+destruct (Sail2_values.mem_bytes_of_bits v); auto.
+Qed.
+Hint Rewrite liftState_write_memt : liftState.
+
+Lemma liftState_write_mem Regs Regval A B E wk addrsize addr sz v r :
+  liftState (Regs := Regs) r (@write_mem Regval A B E wk addrsize addr sz v) = write_memS wk addr sz v.
+unfold write_mem, write_memS, write_memtS.
+destruct (Sail2_values.mem_bytes_of_bits v); simpl; auto.
+Qed.
+Hint Rewrite liftState_write_mem : liftState.
+
+Lemma bindS_rw_left Regs A B E m1 m2 (f : A -> monadS Regs B E) s :
+  m1 s = m2 s ->
+  bindS m1 f s = bindS m2 f s.
+intro H. unfold bindS. rewrite H. reflexivity.
+Qed. 
+
+Lemma liftState_read_reg_readS Regs Regval A E reg get_regval' set_regval' s :
+  (forall s, map_bind reg.(of_regval) (get_regval' reg.(name) s) = Some (reg.(read_from) s)) ->
+  liftState (Regs := Regs) (get_regval', set_regval') (@read_reg _ Regval A E reg) s = readS (fun x => reg.(read_from) (regstate x)) s.
+intros.
+unfold read_reg. simpl. unfold readS.
+erewrite bindS_rw_left. 2: {
+  apply bindS_returnS_left.
+}
+specialize (H (regstate s)).
+destruct (get_regval' _ _) as [v | ]; only 2: discriminate H.
+rewrite bindS_returnS_left.
+simpl in *.
+rewrite H.
+reflexivity.
+Qed.
+
+Lemma liftState_write_reg_updateS Regs Regval A E get_regval' set_regval' reg (v : A) s :
+  (forall s, set_regval' (name reg) (regval_of reg v) s = Some (write_to reg v s)) ->
+  liftState (Regs := Regs) (Regval := Regval) (E := E) (get_regval', set_regval') (write_reg reg v) s = updateS (fun s => {| regstate := (write_to reg v s.(regstate)); memstate := s.(memstate); tagstate := s.(tagstate) |}) s.
+intros.
+unfold write_reg. simpl. unfold readS, seqS.
+erewrite bindS_rw_left. 2: {
+  apply bindS_returnS_left.
+}
+specialize (H (regstate s)).
+destruct (set_regval' _ _) as [v' | ]; only 2: discriminate H.
+injection H as H1.
+unfold updateS.
+rewrite <- H1.
+reflexivity.
+Qed.
+(*
+Lemma liftState_iter_aux Regs Regval A E :
+  liftState r (iter_aux i f xs) = iterS_aux i (fun i x => liftState r (f i x)) xs.
+  by (induction i "\<lambda>i x. liftState r (f i x)" xs rule: iterS_aux.induct)
+     (auto simp: liftState_simp cong: bindS_cong)
+Hint Rewrite liftState_iter_aux : liftState.
+
+lemma liftState_iteri[liftState_simp]:
+  "liftState r (iteri f xs) = iteriS (\<lambda>i x. liftState r (f i x)) xs"
+  by (auto simp: iteri_def iteriS_def liftState_simp)
+
+lemma liftState_iter[liftState_simp]:
+  "liftState r (iter f xs) = iterS (liftState r \<circ> f) xs"
+  by (auto simp: iter_def iterS_def liftState_simp)
+*)
+Lemma liftState_foreachM Regs Regval A Vars E (xs : list A) (vars : Vars) (body : A -> Vars -> monad Regval Vars E) r s :
+  liftState (Regs := Regs) r (foreachM xs vars body) s = foreachS xs vars (fun x vars => liftState r (body x vars)) s.
+revert vars s.
+induction xs as [ | h t].
+* reflexivity.
+* intros vars s. simpl.
+  autorewrite with liftState.
+  apply bindS_ext_cong; auto.
+Qed.
+Hint Rewrite liftState_foreachM : liftState.
+
+Lemma foreachS_cong {A RV Vars E} xs vars f f' s :
+  (forall a vars s, f a vars s = f' a vars s) ->
+  @foreachS A RV Vars E xs vars f s = foreachS xs vars f' s.
+intro H.
+revert s vars.
+induction xs.
+* reflexivity.
+* intros. simpl.
+  apply bindS_ext_cong; auto.
+Qed.
+
+Lemma liftState_genlistM Regs Regval A E r f n s :
+  liftState (Regs := Regs) r (@genlistM A Regval E f n) s = genlistS (fun x => liftState r (f x)) n s.
+unfold genlistM, genlistS.
+autorewrite with liftState.
+apply foreachS_cong.
+intros; autorewrite with liftState.
+apply bindS_ext_cong; auto.
+Qed.
+Hint Rewrite liftState_genlistM : liftState.
+
+Lemma liftState_choose_bools Regs Regval E descr n r s :
+  liftState (Regs := Regs) r (@choose_bools Regval E descr n) s = choose_boolsS n s.
+unfold choose_bools, choose_boolsS.
+autorewrite with liftState.
+reflexivity.
+Qed.
+Hint Rewrite liftState_choose_bools : liftState.
+
+(*
+Lemma liftState_bools_of_bits_nondet[liftState_simp]:
+  "liftState r (bools_of_bits_nondet bs) = bools_of_bits_nondetS bs"
+  unfolding bools_of_bits_nondet_def bools_of_bits_nondetS_def
+  by (auto simp: liftState_simp comp_def)
+Hint Rewrite liftState_choose_bools : liftState.
+*)
+
+Lemma liftState_internal_pick Regs Regval A E r (xs : list A) s :
+  liftState (Regs := Regs) (Regval := Regval) (E := E) r (internal_pick xs) s = internal_pickS xs s.
+unfold internal_pick, internal_pickS.
+unfold choose.
+autorewrite with liftState.
+apply bindS_ext_cong.
+* autorewrite with liftState.
+  reflexivity.
+* intros.
+  destruct (nth_error _ _); auto.
+Qed.
+Hint Rewrite liftState_internal_pick : liftState.
+
+Lemma liftRS_returnS (*[simp]:*) A R Regs E x :
+  @liftRS A R Regs E (returnS x) = returnS x.
+reflexivity.
+Qed.
+
+Lemma concat_singleton A (xs : list A) :
+  concat (xs::nil) = xs.
+simpl.
+rewrite app_nil_r.
+reflexivity.
+Qed.
+
+Lemma liftRS_bindS Regs A B R E (m : monadS Regs A E) (f : A -> monadS Regs B E) s :
+  @liftRS B R Regs E (bindS m f) s = bindS (liftRS m) (fun x => liftRS (f x)) s.
+unfold liftRS, try_catchS, bindS, throwS, returnS.
+induction (m s) as [ | [[a | [msg | e]] t]].
+* reflexivity.
+* simpl. rewrite flat_map_app. rewrite IHl. reflexivity.
+* simpl. rewrite IHl. reflexivity.
+* simpl. rewrite IHl. reflexivity.
+Qed.
+
+Lemma liftRS_assert_expS_True (*[simp]:*) Regs R E msg :
+  @liftRS _ R Regs E (assert_expS true msg) = returnS tt.
+reflexivity.
+Qed.
+
+(*
+lemma untilM_domI:
+  fixes V :: "'vars \<Rightarrow> nat"
+  assumes "Inv vars"
+    and "\<And>vars t vars' t'. \<lbrakk>Inv vars; Run (body vars) t vars'; Run (cond vars') t' False\<rbrakk> \<Longrightarrow> V vars' < V vars \<and> Inv vars'"
+  shows "untilM_dom (vars, cond, body)"
+  using assms
+  by (induction vars rule: measure_induct_rule[where f = V])
+     (auto intro: untilM.domintros)
+
+lemma untilM_dom_untilS_dom:
+  assumes "untilM_dom (vars, cond, body)"
+  shows "untilS_dom (vars, liftState r \<circ> cond, liftState r \<circ> body, s)"
+  using assms
+  by (induction vars cond body arbitrary: s rule: untilM.pinduct)
+     (rule untilS.domintros, auto elim!: Value_liftState_Run)
+
+lemma measure2_induct:
+  fixes f :: "'a \<Rightarrow> 'b \<Rightarrow> nat"
+  assumes "\<And>x1 y1. (\<And>x2 y2. f x2 y2 < f x1 y1 \<Longrightarrow> P x2 y2) \<Longrightarrow> P x1 y1"
+  shows "P x y"
+proof -
+  have "P (fst x) (snd x)" for x
+    by (induction x rule: measure_induct_rule[where f = "\<lambda>x. f (fst x) (snd x)"]) (auto intro: assms)
+  then show ?thesis by auto
+qed
+
+lemma untilS_domI:
+  fixes V :: "'vars \<Rightarrow> 'regs sequential_state \<Rightarrow> nat"
+  assumes "Inv vars s"
+    and "\<And>vars s vars' s' s''.
+           \<lbrakk>Inv vars s; (Value vars', s') \<in> body vars s; (Value False, s'') \<in> cond vars' s'\<rbrakk>
+            \<Longrightarrow> V vars' s'' < V vars s \<and> Inv vars' s''"
+  shows "untilS_dom (vars, cond, body, s)"
+  using assms
+  by (induction vars s rule: measure2_induct[where f = V])
+     (auto intro: untilS.domintros)
+
+lemma whileS_dom_step:
+  assumes "whileS_dom (vars, cond, body, s)"
+    and "(Value True, s') \<in> cond vars s"
+    and "(Value vars', s'') \<in> body vars s'"
+  shows "whileS_dom (vars', cond, body, s'')"
+  by (use assms in \<open>induction vars cond body s arbitrary: vars' s' s'' rule: whileS.pinduct\<close>)
+     (auto intro: whileS.domintros)
+
+lemma whileM_dom_step:
+  assumes "whileM_dom (vars, cond, body)"
+    and "Run (cond vars) t True"
+    and "Run (body vars) t' vars'"
+  shows "whileM_dom (vars', cond, body)"
+  by (use assms in \<open>induction vars cond body arbitrary: vars' t t' rule: whileM.pinduct\<close>)
+     (auto intro: whileM.domintros)
+
+lemma whileM_dom_ex_step:
+  assumes "whileM_dom (vars, cond, body)"
+    and "\<exists>t. Run (cond vars) t True"
+    and "\<exists>t'. Run (body vars) t' vars'"
+  shows "whileM_dom (vars', cond, body)"
+  using assms by (blast intro: whileM_dom_step)
+
+lemmas whileS_pinduct = whileS.pinduct[case_names Step]
+
+lemma liftState_whileM:
+  assumes "whileS_dom (vars, liftState r \<circ> cond, liftState r \<circ> body, s)"
+    and "whileM_dom (vars, cond, body)"
+  shows "liftState r (whileM vars cond body) s = whileS vars (liftState r \<circ> cond) (liftState r \<circ> body) s"
+proof (use assms in \<open>induction vars "liftState r \<circ> cond" "liftState r \<circ> body" s rule: whileS.pinduct\<close>)
+  case Step: (1 vars s)
+  note domS = Step(1) and IH = Step(2) and domM = Step(3)
+  show ?case unfolding whileS.psimps[OF domS] whileM.psimps[OF domM] liftState_bind
+  proof (intro bindS_ext_cong, goal_cases cond while)
+    case (while a s')
+    have "bindS (liftState r (body vars)) (liftState r \<circ> (\<lambda>vars. whileM vars cond body)) s' =
+          bindS (liftState r (body vars)) (\<lambda>vars. whileS vars (liftState r \<circ> cond) (liftState r \<circ> body)) s'"
+      if "a"
+    proof (intro bindS_ext_cong, goal_cases body while')
+      case (while' vars' s'')
+      have "whileM_dom (vars', cond, body)" proof (rule whileM_dom_ex_step[OF domM])
+        show "\<exists>t. Run (cond vars) t True" using while that by (auto elim: Value_liftState_Run)
+        show "\<exists>t'. Run (body vars) t' vars'" using while' that by (auto elim: Value_liftState_Run)
+      qed
+      then show ?case using while while' that IH by auto
+    qed auto
+    then show ?case by (auto simp: liftState_simp)
+  qed auto
+qed
+
+
+lemma untilM_dom_step:
+  assumes "untilM_dom (vars, cond, body)"
+    and "Run (body vars) t vars'"
+    and "Run (cond vars') t' False"
+  shows "untilM_dom (vars', cond, body)"
+  by (use assms in \<open>induction vars cond body arbitrary: vars' t t' rule: untilM.pinduct\<close>)
+     (auto intro: untilM.domintros)
+
+lemma untilM_dom_ex_step:
+  assumes "untilM_dom (vars, cond, body)"
+    and "\<exists>t. Run (body vars) t vars'"
+    and "\<exists>t'. Run (cond vars') t' False"
+  shows "untilM_dom (vars', cond, body)"
+  using assms by (blast intro: untilM_dom_step)
+
+lemma liftState_untilM:
+  assumes "untilS_dom (vars, liftState r \<circ> cond, liftState r \<circ> body, s)"
+    and "untilM_dom (vars, cond, body)"
+  shows "liftState r (untilM vars cond body) s = untilS vars (liftState r \<circ> cond) (liftState r \<circ> body) s"
+proof (use assms in \<open>induction vars "liftState r \<circ> cond" "liftState r \<circ> body" s rule: untilS.pinduct\<close>)
+  case Step: (1 vars s)
+  note domS = Step(1) and IH = Step(2) and domM = Step(3)
+  show ?case unfolding untilS.psimps[OF domS] untilM.psimps[OF domM] liftState_bind
+  proof (intro bindS_ext_cong, goal_cases body k)
+    case (k vars' s')
+    show ?case unfolding comp_def liftState_bind
+    proof (intro bindS_ext_cong, goal_cases cond until)
+      case (until a s'')
+      have "untilM_dom (vars', cond, body)" if "\<not>a"
+      proof (rule untilM_dom_ex_step[OF domM])
+        show "\<exists>t. Run (body vars) t vars'" using k by (auto elim: Value_liftState_Run)
+        show "\<exists>t'. Run (cond vars') t' False" using until that by (auto elim: Value_liftState_Run)
+      qed
+      then show ?case using k until IH by (auto simp: comp_def liftState_simp)
+    qed auto
+  qed auto
+qed
+
+text \<open>Simplification rules for monadic Boolean connectives\<close>
+
+lemma if_return_return[simp]: "(if a then return True else return False) = return a" by auto
+
+lemma and_boolM_simps[simp]:
+  "and_boolM (return b) (return c) = return (b \<and> c)"
+  "and_boolM x (return True) = x"
+  "and_boolM x (return False) = x \<bind> (\<lambda>_. return False)"
+  "\<And>x y z. and_boolM (x \<bind> y) z = (x \<bind> (\<lambda>r. and_boolM (y r) z))"
+  by (auto simp: and_boolM_def)
+
+lemma and_boolM_return_if:
+  "and_boolM (return b) y = (if b then y else return False)"
+  by (auto simp: and_boolM_def)
+
+lemma and_boolM_return_return_and[simp]: "and_boolM (return l) (return r) = return (l \<and> r)"
+  by (auto simp: and_boolM_def)
+
+lemmas and_boolM_if_distrib[simp] = if_distrib[where f = "\<lambda>x. and_boolM x y" for y]
+
+lemma or_boolM_simps[simp]:
+  "or_boolM (return b) (return c) = return (b \<or> c)"
+  "or_boolM x (return True) = x \<bind> (\<lambda>_. return True)"
+  "or_boolM x (return False) = x"
+  "\<And>x y z. or_boolM (x \<bind> y) z = (x \<bind> (\<lambda>r. or_boolM (y r) z))"
+  by (auto simp: or_boolM_def)
+
+lemma or_boolM_return_if:
+  "or_boolM (return b) y = (if b then return True else y)"
+  by (auto simp: or_boolM_def)
+
+lemma or_boolM_return_return_or[simp]: "or_boolM (return l) (return r) = return (l \<or> r)"
+  by (auto simp: or_boolM_def)
+
+lemmas or_boolM_if_distrib[simp] = if_distrib[where f = "\<lambda>x. or_boolM x y" for y]
+
+lemma if_returnS_returnS[simp]: "(if a then returnS True else returnS False) = returnS a" by auto
+
+lemma and_boolS_simps[simp]:
+  "and_boolS (returnS b) (returnS c) = returnS (b \<and> c)"
+  "and_boolS x (returnS True) = x"
+  "and_boolS x (returnS False) = bindS x (\<lambda>_. returnS False)"
+  "\<And>x y z. and_boolS (bindS x y) z = (bindS x (\<lambda>r. and_boolS (y r) z))"
+  by (auto simp: and_boolS_def)
+
+lemma and_boolS_returnS_if:
+  "and_boolS (returnS b) y = (if b then y else returnS False)"
+  by (auto simp: and_boolS_def)
+
+lemmas and_boolS_if_distrib[simp] = if_distrib[where f = "\<lambda>x. and_boolS x y" for y]
+
+lemma and_boolS_returnS_True[simp]: "and_boolS (returnS True) c = c"
+  by (auto simp: and_boolS_def)
+
+lemma or_boolS_simps[simp]:
+  "or_boolS (returnS b) (returnS c) = returnS (b \<or> c)"
+  "or_boolS (returnS False) m = m"
+  "or_boolS x (returnS True) = bindS x (\<lambda>_. returnS True)"
+  "or_boolS x (returnS False) = x"
+  "\<And>x y z. or_boolS (bindS x y) z = (bindS x (\<lambda>r. or_boolS (y r) z))"
+  by (auto simp: or_boolS_def)
+
+lemma or_boolS_returnS_if:
+  "or_boolS (returnS b) y = (if b then returnS True else y)"
+  by (auto simp: or_boolS_def)
+
+lemmas or_boolS_if_distrib[simp] = if_distrib[where f = "\<lambda>x. or_boolS x y" for y]
+
+lemma Run_or_boolM_E:
+  assumes "Run (or_boolM l r) t a"
+  obtains "Run l t True" and "a"
+  | tl tr where "Run l tl False" and "Run r tr a" and "t = tl @ tr"
+  using assms by (auto simp: or_boolM_def elim!: Run_bindE Run_ifE Run_returnE)
+
+lemma Run_and_boolM_E:
+  assumes "Run (and_boolM l r) t a"
+  obtains "Run l t False" and "\<not>a"
+  | tl tr where "Run l tl True" and "Run r tr a" and "t = tl @ tr"
+  using assms by (auto simp: and_boolM_def elim!: Run_bindE Run_ifE Run_returnE)
+
+lemma maybe_failS_Some[simp]: "maybe_failS msg (Some v) = returnS v"
+  by (auto simp: maybe_failS_def)
+
+text \<open>Event traces\<close>
+
+lemma Some_eq_bind_conv: "Some x = Option.bind f g \<longleftrightarrow> (\<exists>y. f = Some y \<and> g y = Some x)"
+  unfolding bind_eq_Some_conv[symmetric] by auto
+
+lemma if_then_Some_eq_Some_iff: "((if b then Some x else None) = Some y) \<longleftrightarrow> (b \<and> y = x)"
+  by auto
+
+lemma Some_eq_if_then_Some_iff: "(Some y = (if b then Some x else None)) \<longleftrightarrow> (b \<and> y = x)"
+  by auto
+
+lemma emitEventS_update_cases:
+  assumes "emitEventS ra e s = Some s'"
+  obtains
+    (Write_mem) wk addr sz v tag r
+      where "e = E_write_memt wk addr sz v tag r \<or> (e = E_write_mem wk addr sz v r \<and> tag = B0)"
+        and "s' = put_mem_bytes addr sz v tag s"
+  | (Write_reg) r v rs'
+      where "e = E_write_reg r v" and "(snd ra) r v (regstate s) = Some rs'"
+        and "s' = s\<lparr>regstate := rs'\<rparr>"
+  | (Read) "s' = s"
+  using assms
+  by (elim emitEventS.elims)
+     (auto simp: Some_eq_bind_conv bind_eq_Some_conv if_then_Some_eq_Some_iff Some_eq_if_then_Some_iff)
+
+lemma runTraceS_singleton[simp]: "runTraceS ra [e] s = emitEventS ra e s"
+  by (cases "emitEventS ra e s"; auto)
+
+lemma runTraceS_ConsE:
+  assumes "runTraceS ra (e # t) s = Some s'"
+  obtains s'' where "emitEventS ra e s = Some s''" and "runTraceS ra t s'' = Some s'"
+  using assms by (auto simp: bind_eq_Some_conv)
+
+lemma runTraceS_ConsI:
+  assumes "emitEventS ra e s = Some s'" and "runTraceS ra t s' = Some s''"
+  shows "runTraceS ra (e # t) s = Some s''"
+  using assms by auto
+
+lemma runTraceS_Cons_tl:
+  assumes "emitEventS ra e s = Some s'"
+  shows "runTraceS ra (e # t) s = runTraceS ra t s'"
+  using assms by (elim emitEventS.elims) (auto simp: Some_eq_bind_conv bind_eq_Some_conv)
+
+lemma runTraceS_appendE:
+  assumes "runTraceS ra (t @ t') s = Some s'"
+  obtains s'' where "runTraceS ra t s = Some s''" and "runTraceS ra t' s'' = Some s'"
+proof -
+  have "\<exists>s''. runTraceS ra t s = Some s'' \<and> runTraceS ra t' s'' = Some s'"
+  proof (use assms in \<open>induction t arbitrary: s\<close>)
+    case (Cons e t)
+    from Cons.prems
+    obtain s_e where "emitEventS ra e s = Some s_e" and "runTraceS ra (t @ t') s_e = Some s'"
+      by (auto elim: runTraceS_ConsE simp: bind_eq_Some_conv)
+    with Cons.IH[of s_e] show ?case by (auto intro: runTraceS_ConsI)
+  qed auto
+  then show ?thesis using that by blast
+qed
+
+lemma runTraceS_nth_split:
+  assumes "runTraceS ra t s = Some s'" and n: "n < length t"
+  obtains s1 s2 where "runTraceS ra (take n t) s = Some s1"
+    and "emitEventS ra (t ! n) s1 = Some s2"
+    and "runTraceS ra (drop (Suc n) t) s2 = Some s'"
+proof -
+  have "runTraceS ra (take n t @ t ! n # drop (Suc n) t) s = Some s'"
+    using assms
+    by (auto simp: id_take_nth_drop[OF n, symmetric])
+  then show thesis by (blast elim: runTraceS_appendE runTraceS_ConsE intro: that)
+qed
+
+text \<open>Memory accesses\<close>
+
+lemma get_mem_bytes_put_mem_bytes_same_addr:
+  assumes "length v = sz"
+  shows "get_mem_bytes addr sz (put_mem_bytes addr sz v tag s) = Some (v, if sz > 0 then tag else B1)"
+proof (unfold assms[symmetric], induction v rule: rev_induct)
+  case Nil
+  then show ?case by (auto simp: get_mem_bytes_def)
+next
+  case (snoc x xs)
+  then show ?case
+    by (cases tag)
+       (auto simp: get_mem_bytes_def put_mem_bytes_def Let_def and_bit_eq_iff foldl_and_bit_eq_iff
+             cong: option.case_cong split: if_splits option.splits)
+qed
+
+lemma memstate_put_mem_bytes:
+  assumes "length v = sz"
+  shows "memstate (put_mem_bytes addr sz v tag s) addr' =
+         (if addr' \<in> {addr..<addr+sz} then Some (v ! (addr' - addr)) else memstate s addr')"
+  unfolding assms[symmetric]
+  by (induction v rule: rev_induct) (auto simp: put_mem_bytes_def nth_Cons nth_append Let_def)
+
+lemma tagstate_put_mem_bytes:
+  assumes "length v = sz"
+  shows "tagstate (put_mem_bytes addr sz v tag s) addr' =
+         (if addr' \<in> {addr..<addr+sz} then Some tag else tagstate s addr')"
+  unfolding assms[symmetric]
+  by (induction v rule: rev_induct) (auto simp: put_mem_bytes_def nth_Cons nth_append Let_def)
+
+lemma get_mem_bytes_cong:
+  assumes "\<forall>addr'. addr \<le> addr' \<and> addr' < addr + sz \<longrightarrow>
+                   (memstate s' addr' = memstate s addr' \<and> tagstate s' addr' = tagstate s addr')"
+  shows "get_mem_bytes addr sz s' = get_mem_bytes addr sz s"
+proof (use assms in \<open>induction sz\<close>)
+  case 0
+  then show ?case by (auto simp: get_mem_bytes_def)
+next
+  case (Suc sz)
+  then show ?case
+    by (auto simp: get_mem_bytes_def Let_def
+             intro!: map_option_cong map_cong foldl_cong
+                     arg_cong[where f = just_list] arg_cong2[where f = and_bit])
+qed
+
+lemma get_mem_bytes_tagged_tagstate:
+  assumes "get_mem_bytes addr sz s = Some (v, B1)"
+  shows "\<forall>addr' \<in> {addr..<addr + sz}. tagstate s addr' = Some B1"
+  using assms
+  by (auto simp: get_mem_bytes_def foldl_and_bit_eq_iff Let_def split: option.splits)
+
+end
+*)
